The function of the untouched string

$y_{\textrm{nof}}(t) = y_{\textrm{in}}(t-\lfloor\frac{t}{T_N}\rfloor T_N)R_N^{\lfloor\frac{t}{T_N}\rfloor}$
(\ref{eq:rho0})

is part of the explicit formula of the touched string (\ref{eq:explicit}),
this relationship can 

forward in time by $-kT_F$

$y_{\textrm{nof}}(t-kT_F) = y_{\textrm{in}}(t-kT_F-\mmm T_N)R_N^{\mmm}$

and using $m=\mmm$ to obtain

$y_{\textrm{nof}}(t-kT_F) = y_{\textrm{in}}(t-kT_F-m T_N)R_N^{m}$.

In this form it is easy to recognize $y_{\textrm{nof}}$ inside

$y_{\textrm{out}}(t) = \sum_{k=0}^{\lfloor \frac{t}{T_F} \rfloor}\left(y_{\textrm{in}}(t - kT_F - mT_N)\binom{m+k}{k} (1 - \rho)^{k} \rho^mR_N^mR_F^k\right)$
(\ref{eq:explicit})

and substituted with $y_{\textrm{nof}}(t-kT_F)$, resulting in

$y_{\textrm{out}}(t) = \sum_{k=0}^{\lfloor \frac{t}{T_F} \rfloor}\left(y_{\textrm{nof}}(t - kT_F)\binom{m+k}{k} (1 - \rho)^{k} \rho^mR_F^k\right)$.
