Starting from the expression of the untouched string

$y_{\textrm{nof}}(t) = y_{\textrm{in}}((\frac{t}{T_N}-\lfloor\frac{t}{T_N}\rfloor)T_N)R_N^{\lfloor\frac{t}{T_N}\rfloor}$,

we give a separate definition to the lossless part of the untouched string's function, as follows

$y_{\textrm{nol}}(t) = y_{\textrm{in}}((\frac{t}{T_N}-\lfloor\frac{t}{T_N}\rfloor)T_N)$,

and rewriting $y_{\textrm{nof}}$ accordingly

$y_{\textrm{nof}}(t) = y_{\textrm{nol}}(t)R_N^{\lfloor\frac{t}{T_N}\rfloor}$.

Assuming that $R=R_F=R_N$

$y_{\textrm{out}}(t) = \sum_{k=0}^{\lfloor \frac{t}{T_F} \rfloor}\left(y_{\textrm{nol}}(t - kT_F)\binom{m+k}{k} (1 - \rho)^{k} \rho^mR_N^{m}R_F^k\right)=$


$\sum_{k=0}^{\lfloor \frac{t}{T_F} \rfloor}\left(y_{\textrm{nol}}(t - kT_F)\binom{m+k}{k} (1 - \rho)^{k} \rho^mR^{m+k}\right)=$

$\sum_{k=0}^{\lfloor \frac{t}{T_F} \rfloor}\left(y_{\textrm{nol}}(t - kT_F)\binom{m+k}{k} (1 - \rho)^{k} \rho^mR^{\mmm+k}\right)=$

$\sum_{k=0}^{\lfloor \frac{t}{T_F} \rfloor}\left(y_{\textrm{nol}}(t - kT_F)\binom{m+k}{k} (1 - \rho)^{k} \rho^mR^{\left\lfloor \frac{t - kT_F + kT_N}{T_N} \right\rfloor}\right)=$

$\sum_{k=0}^{\lfloor \frac{t}{T_F} \rfloor}\left(y_{\textrm{nol}}(t - kT_F + kT_N)\binom{m+k}{k} (1 - \rho)^{k} \rho^mR^{\left\lfloor \frac{t - kT_F + kT_N}{T_N} \right\rfloor}\right)=$

$\sum_{k=0}^{\lfloor \frac{t}{T_F} \rfloor}\left(y_{\textrm{nof}}(t - kT_F + kT_N)\binom{m+k}{k} (1 - \rho)^{k} \rho^m\right)$
