
$\sum_{k=0}^{\lfloor \frac{n}{T_F} \rfloor}\left(y[n - (kT_F + mT_N)]\binom{m+k}{k} (1 - \rho)^{k} \rho^mR_N^mR_F^k\right)=$

$\sum_{k=0}^{\lfloor \frac{n}{T_F} \rfloor}\left(y[n - kT_F - \left\lfloor \frac{n - kT_F}{T_N} \right\rfloor T_N)]\binom{m+k}{k} (1 - \rho)^{k} \rho^mR_N^{\left\lfloor \frac{n - kT_F}{T_N} \right\rfloor}R_F^k\right)=$

$\sum_{k=0}^{\lfloor \frac{n}{T_F} \rfloor}\left(y[(\frac{n - kT_F}{T_N} - \left\lfloor \frac{n - kT_F}{T_N} \right\rfloor) T_N]\binom{m+k}{k} (1 - \rho)^{k} \rho^mR_N^{\left\lfloor \frac{n - kT_F}{T_N} \right\rfloor}R_F^k\right)$

The formula $y_0[n]$ of the untouched string can be obtained by setting $\rho=1$

$y_0[n] = y[(\frac{n}{T_N}-\lfloor\frac{n}{T_N}\rfloor)T_N]R_N^{\lfloor\frac{n}{T_N}\rfloor}$

The argument of $y$ has the form of a sawtooth wave with a frequency of $T_N$

$y_0[n] = y_{ls}[n]R_N^{\lfloor\frac{n}{T_N}\rfloor}$

$\sum_{k=0}^{\lfloor \frac{n}{T_F} \rfloor}\left(y_{ls}[n - kT_F]\binom{m+k}{k} (1 - \rho)^{k} \rho^mR_N^{\left\lfloor \frac{n - kT_F}{T_N} \right\rfloor}R_F^k\right)=$

We assume that $R_F=R_N$

$\sum_{k=0}^{\lfloor \frac{n}{T_F} \rfloor}\left(y_{ls}[n - kT_F]\binom{m+k}{k} (1 - \rho)^{k} \rho^mR_N^{\left\lfloor \frac{n - kT_F}{T_N} \right\rfloor+k}\right)=$

$\sum_{k=0}^{\lfloor \frac{n}{T_F} \rfloor}\left(y_{ls}[n - kT_F]\binom{m+k}{k} (1 - \rho)^{k} \rho^mR_N^{\left\lfloor \frac{n - kT_F + kT_N}{T_N} \right\rfloor}\right)=$

$\sum_{k=0}^{\lfloor \frac{n}{T_F} \rfloor}\left(y_{ls}[n - kT_F + kT_N]\binom{m+k}{k} (1 - \rho)^{k} \rho^mR_N^{\left\lfloor \frac{n - kT_F + kT_N}{T_N} \right\rfloor}\right)=$

$\sum_{k=0}^{\lfloor \frac{n}{T_F} \rfloor}\left(y_0[n - kT_F + kT_N]\binom{m+k}{k} (1 - \rho)^{k} \rho^m\right)$
